finalizing

src/cruft.v
@@ -320,3 +320,221 @@ Check H0.
                 it resulted in the same 3 updates to the reigsters map *)
             reflexivity.
         Qed.
+
+
+
+  
+(* r3 := 4*)
+Definition bb0 : block (fin 1) := 
+  after [
+      Imov 3 (Oimm 4)
+  ] (Bhalt).
+  
+  (* r3 := r1 + r2*)
+  Definition bb1 : block (fin 1) := 
+  after [
+      Iadd 3 1 (Oreg 2)
+  ] (Bhalt).
+  (*  Try to show that these instructions are bisimilar
+  
+   i1:   r3 := 4
+  
+   i2:   r3 := r1 + r2
+  *)
+  Definition i1 : instr 
+      := Iadd 3 1 (Oreg 2).
+  
+  Definition i2 : instr 
+      := Iadd 3 2 (Oreg 1).
+  
+  (*
+     we can denote each instruction as Itrees using some 
+     effect type E where the types of effects we have are
+  
+     E:= 
+      | GetReg 
+      | SetReg 
+      | Load
+      | Store
+      | Done 
+     *)
+  Notation E := Utils.utils.E.
+  
+  Definition itree_i1 : itree E _ := denote_instr i1.
+  Definition itree_i2 : itree E _ := denote_instr i2.
+  
+  Remark CantProve : 
+      itree_i1
+  ≈
+      itree_i2.
+   (* comptue the denotation of both instructions as itrees *)
+   unfold itree_i1; unfold itree_i2; unfold denote_instr ; simpl.
+   (* try to peel off the first GetReg *)
+   eutt_clo_bind_eq.
+   (* stuck !*)
+   Abort.
+  
+  (* The problem is that GetReg and SetReg "mean" something..
+     
+     we have GetReg and SetReg effects.. 
+     but we need to run them through an effect handler
+  
+     thats what interp_asm is for!
+     *)
+  Check interp_asm.
+  Print interp_asm.
+  
+  Definition interpret {E' A} :
+      (memory) ->
+      (registers) ->
+      itree (Reg +' Memory +' E') A  ->
+      itree E' (memory * (registers * A))
+   := 
+      fun m r prog => 
+          interp_asm prog m r.
+  
+  (*
+      interp_asm is is the effect handler for asm programs
+      it maps GetReg and SetReg to concrete implementations via 
+      the register handler h_reg
+  
+      h_reg := 
+          GetReg x => lookup_def x
+        | SetReg x v => insert x v
+  
+  *)
+  Print h_reg.
+  
+  
+  (* We can see if 
+      i1:   r3 := r1 + r2
+  
+      i2:   r3 := r2 + r1 
+      
+    are bisimilar when we interpret GetReg and SetReg 
+  
+    to do that, we need to specify the initial memory 
+      and register configuration
+  
+  
+   lets say the initial memory is empty 
+     and that the initial registers are 
+          r1 := 2 
+          r2 := 3
+          
+  
+      then the final memory is still empty
+      and the final registers are 
+          r1 := 2
+          r2 := 3
+          r3 := 5
+          *)
+  
+  Definition mem : memory := [].
+  Definition startReg : registers := 
+  [
+      (1,2);
+      (2,3)
+  ].
+  Definition endReg : registers := 
+  [
+      (3,5);
+      (1,2);
+      (2,3)
+  ].
+  
+  Definition result {E} : itree E (memory * (registers * unit))
+      := Ret (mem , (endReg , tt)).
+  
+  Notation "x ≋ y" := ((eutt rel_asm) x y)(at level 50).
+  
+  Notation denote_instr := (Asm.denote_instr (E := E)).
+  
+  Compute interp_asm (denote_instr i1).
+  (* we need to interpret these instructions! *)
+  Example interpret_i1 : 
+      interp_asm (denote_instr i1) mem startReg 
+      ≋ 
+      result.
+  
+      (* first denote instruction 1 as an itree*)
+      unfold i1.
+      unfold denote_instr ; simpl.
+      (* then start interpreting the events *)
+      rewrite interp_asm_GetReg.
+      rewrite interp_asm_GetReg; simpl.
+      rewrite interp_asm_SetReg'; cbn.
+      (* now all the events have been interpreted 
+          see if it equals the result *)
+      unfold result.
+      unfold startReg.
+      unfold alist_add; unfold alist_remove; simpl.
+      unfold endReg.
+      (* the results match! *)
+      reflexivity.
+  Qed.
+    
+  
+  
+  (* To do that we are going to put i1 and i2 in their own basic blocks*)
+  (* 
+      bb0:
+          r3 := r1 + r2
+  *)
+  Definition bb0 : block (fin 1) := 
+  after [
+      Iadd 3 1 (Oreg 2)
+  ] (Bhalt).
+  
+  (* 
+      bb1:
+          r3 := r2 + r1
+  *)
+  Definition bb1 : block (fin 1) := 
+  after [
+      Iadd 3 2 (Oreg 1)
+  ] (Bhalt).
+  
+  (* then we turn those blocks into itrees *)
+  Definition bb0_itree : itree E (fin 1) 
+    := denote_asm (raw_asm_block bb0) f0.
+  
+  Definition bb1_itree : itree E (fin 1) 
+    := denote_asm (raw_asm_block bb1) f0.
+  
+  (* but what does bb0 look like as an itree? 
+  lets explore that by stepping through the denotation *)
+  Lemma den_bb0 : 
+      bb0_itree 
+  ≈   
+  (   lv <- trigger (GetReg 1);;
+      rv <- trigger (GetReg 2);;
+      trigger (SetReg 3 (lv + rv)));; 
+      exit.
+  Proof.
+     unfold bb0_itree.
+      setoid_rewrite raw_asm_block_correct.
+      unfold bb0.
+      simpl.
+      reflexivity.
+  Qed.
+  
+  (*based on that exercise 
+      we can see what bb1 is as an itree *)
+  Lemma den_bb1 : 
+      bb1_itree 
+  ≈   
+  (  
+      lv <- trigger (GetReg 2);;
+      rv <- trigger (GetReg 1);;
+      trigger (SetReg 3 (lv + rv)));; 
+      exit.
+  Proof.
+   (* lets just use a custom tactic to do this *)
+   denBlock bb1_itree bb1.
+  Qed.
+  
+  
+  
+      
+  
