src/demo/Utils.v
@@ -1,0 +1,162 @@
+From Coq Require Import
+Lists.List
+Strings.String
+Morphisms
+ZArith
+Setoid
+RelationClasses.
+
+(*Turning off some of the notation 
+helps to see what rules might be helpful*)
+
+From ITree Require Import
+    Eq.Eqit
+    Basics.Category
+    Basics.HeterogeneousRelations
+    Basics.Monad
+    Basics.CategorySub
+    Basics.CategoryOps
+    Interp.InterpFacts
+    Events.MapDefault
+    Events.MapDefaultFacts
+    Events.State
+    Events.StateFacts
+    ITreeMonad
+    ITreeFacts
+    ITree.
+
+From ExtLib Require Import
+    Core.RelDec
+    Structures.Monad
+    Structures.Maps
+    Programming.Show
+    Data.Map.FMapAList.
+
+Import CatNotations.
+Local Open Scope cat_scope.
+Local Open Scope itree_scope.
+
+From ITreeTutorial Require Import 
+    Fin 
+    Asm 
+    AsmCombinators 
+    AsmOptimization
+    Imp2Asm
+    KTreeFin
+    Utils_tutorial.
+
+Import ITreeNotations.
+
+Import ListNotations.
+Open Scope string_scope.
+
+Import CatNotations.
+Local Open Scope cat_scope.
+Local Open Scope itree_scope.
+
+From ITreeTutorial Require Import Fin Asm AsmCombinators Utils_tutorial.
+
+Module utils.
+
+
+(* definitions *)
+(*
+Context {E : Type -> Type}.
+Context {HasRegs : Reg -< E}.
+Context {HasMemory : Memory -< E}.
+Context {HasExit : Exit -< E}.
+
+
+
+(* notation *)
+Notation denote_instr := (denote_instr (E := E)).
+Notation denote_bk := (denote_bk (E := E)).
+Notation denote_bks := (denote_bks (E := E)).
+Notation denote_asm := (denote_asm (E := E)).
+*)
+Context {E' : Type -> Type}.
+Context {HasRegs : Reg -< E'}.
+Context {HasMemory : Memory -< E'}.
+Context {HasExit : Exit -< E'}.
+    
+Definition E := Reg +' Memory +' Exit +' E'.
+
+Notation denote_bk := (denote_bk (E := E)).
+Notation denote_bks := (denote_bks (E := E)).
+Notation denote_asm := (denote_asm (E := E)).
+Notation "x ≋ y" := ((@eutt E _ _  rel_asm) x y)(at level 50).
+
+(* helper lemmas *)
+Lemma seq_asm_correct {A B C} (ab : asm A B) (bc : asm B C) :
+      denote_asm (seq_asm ab bc)
+    ⩯ denote_asm ab >>> denote_asm bc.
+  Proof.
+    unfold seq_asm.
+    rewrite loop_asm_correct, relabel_asm_correct, app_asm_correct.
+    rewrite fmap_id0, cat_id_r, fmap_swap.
+    apply cat_from_loop.
+  Qed.
+
+Lemma pointfree (p: asm 1 1)(t :ktree_fin E 1 1) :
+    denote_asm p ⩯ t ->
+    denote_asm p f0 ≈ t f0.
+Admitted.
+
+Lemma pointed (k1 k2 :ktree_fin E 1 1) :
+     k1 f0 ≈ k2 f0 ->
+    k1 ⩯ k2.
+Admitted.
+
+(* custom tactics *)
+
+Ltac eutt_clo_bind_eq := 
+        apply (@eutt_clo_bind _ _ _ _ _ _ eq).
+
+Global Hint Extern 1 => eutt_clo_bind_eq : myHints.
+
+Ltac denBlock a_bb bb := 
+    unfold a_bb;
+    setoid_rewrite raw_asm_block_correct;
+    unfold bb;
+    reflexivity.
+
+
+
+(* manually evaluating things can get annoying
+    so we can automate that with metaprogramming / tactics!
+*)
+Ltac getsetRegMem := 
+    match goal with 
+    (* get reg *)
+    | |- (interp_asm 
+           (_ <- trigger (GetReg _);; _)  _ _)
+           ≋ _
+        => setoid_rewrite interp_asm_GetReg
+    | |-    _ ≋ 
+            (interp_asm 
+                (_ <- trigger (GetReg _);; _) 
+                _ _)
+        => setoid_rewrite interp_asm_GetReg
+    (* set reg *)
+    | |-    (interp_asm
+                (trigger (SetReg _ _);; _) _ _ )
+            ≋ _
+        => setoid_rewrite interp_asm_SetReg
+    | |- 
+            _ ≋
+            (interp_asm
+                (trigger (SetReg _ _);; _)  _ _ )
+            
+    => setoid_rewrite interp_asm_SetReg
+    end.
+
+Ltac eval_interp' :=
+        getsetRegMem
+    ||
+        setoid_rewrite bind_ret_ 
+    ||
+        setoid_rewrite bind_bind.
+    
+Ltac eval_interp := 
+    repeat eval_interp'.
+End utils.
