src/demo/bisimilarInstructions.v
@@ -1,0 +1,261 @@
+From Coq Require Import
+Lists.List
+Strings.String
+Morphisms
+Nat
+ZArith
+Setoid
+RelationClasses.
+
+(*Turning off some of the notation 
+helps to see what rules might be helpful*)
+
+From ITree Require Import
+    Eq.Eqit
+    Basics.Category
+    Basics.HeterogeneousRelations
+    Basics.Monad
+    Basics.CategorySub
+    Basics.CategoryOps
+    Interp.InterpFacts
+    Events.MapDefault
+    Events.MapDefaultFacts
+    Events.State
+    Events.StateFacts
+    ITreeMonad
+    ITreeFacts
+    ITree.
+
+From ExtLib Require Import
+    Core.RelDec
+    Structures.Monad
+    Structures.Maps
+    Programming.Show
+    Data.Map.FMapAList.
+
+Import CatNotations.
+Local Open Scope cat_scope.
+Local Open Scope itree_scope.
+
+From ITreeTutorial Require Import 
+    Fin 
+    Asm 
+    AsmCombinators 
+    AsmOptimization
+    Imp2Asm
+    KTreeFin
+    Utils_tutorial.
+
+Import ITreeNotations.
+
+Import ListNotations.
+Open Scope string_scope.
+
+Import CatNotations.
+Local Open Scope cat_scope.
+Local Open Scope itree_scope.
+
+From ITreeTutorial Require Import Fin Asm AsmCombinators Utils_tutorial.
+
+From MyProject Require Import 
+    Utils.
+
+Notation E := Utils.utils.E.
+
+Module bisimilar_instruction.
+Import utils.
+
+Lemma interp_asm_SetReg' {E}  r v mem reg :
+  @eutt E _ _ (rel_asm)
+       (interp_asm (trigger (SetReg r v)) mem reg)
+       (Ret (mem, ((Maps.add r v reg),tt))).
+Admitted.
+
+(*  Try to show that these instructions are bisimilar
+
+ i1:   r3 := r1 + r2
+
+ i2:   r3 := r2 + r1
+*)
+Definition i1 : instr 
+    := Iadd 3 1 (Oreg 2).
+
+Definition i2 : instr 
+    := Iadd 3 2 (Oreg 1).
+
+(*
+   we can denote each instruction as Itrees using some 
+   effect type E where the types of effects we have are
+
+   E:= 
+    | GetReg 
+    | SetReg 
+    | Load
+    | Store
+    | Done 
+   *)
+
+Definition itree_i1 : itree E _ := denote_instr i1.
+Definition itree_i2 : itree E _ := denote_instr i2.
+
+(* 
+ i1:   r3 := r1 + r2
+
+ i2:   r3 := r2 + r1
+
+ It seems like we should be able to say that these to instructions
+ are bisimilar..
+ let's try..
+*)
+Remark CantProve : 
+    itree_i1
+≈
+    itree_i2.
+ (* comptue the denotation of both instructions as itrees *)
+ unfold itree_i1; unfold itree_i2; unfold denote_instr ; simpl.
+ (* try to peel off the first GetReg *)
+ eutt_clo_bind_eq.
+ (* stuck !
+ trigger (GetReg 1) ≈ trigger (GetReg 2)
+ no way to prove this without saying what GetReg does!
+ *)
+ Abort.
+
+(* The problem is that GetReg and SetReg "mean" something..
+   
+   we have GetReg and SetReg effects.. 
+   but we need to run them through an effect handler
+
+   thats what interp_asm is for!
+   *)
+Check interp_asm.
+Print interp_asm.
+
+Definition interpret {E' A} :
+    (memory) ->
+    (registers) ->
+    itree (Reg +' Memory +' E') A  ->
+    itree E' (memory * (registers * A))
+ := 
+    fun m r prog => 
+        interp_asm prog m r.
+
+(*
+    interp_asm is is the effect handler for asm programs
+    it maps GetReg and SetReg to concrete implementations via 
+    the register handler h_reg
+
+    h_reg := 
+        GetReg x => lookup_def x
+      | SetReg x v => insert x v
+
+*)
+Print h_reg.
+
+
+(* We can see if 
+    i1:   r3 := r1 + r2
+
+    i2:   r3 := r2 + r1 
+    
+  are bisimilar when we interpret GetReg and SetReg 
+
+  to do that, we need to specify the initial memory 
+    and register configuration
+
+  these instructions do not modify memory
+    so the initial and final memory maps are the same
+
+ lets say  the initial registers are 
+        r1 := x 
+        r2 := y
+        
+
+ then the final registers are 
+        r1 := x
+        r2 := y
+        r3 := x + y OR y + x // depending on i1 or i2
+        *)
+(* summon some variables*)
+Variable x : nat.
+Variable y : nat.
+Variable mem : memory.
+
+Definition startReg : registers := 
+[
+    (1,x);
+    (2,y)
+].
+Definition endReg_i1 : registers := 
+[
+    (3,x + y);
+    (1,x);
+    (2,y)
+].
+
+Definition result_i1 {E} : itree E (memory * (registers * unit))
+    := Ret (mem , (endReg_i1 , tt)).
+
+
+
+(* 
+lets check that 
+    i1 := r3 := r1 + r2
+when
+    r1 := x
+    r2 := y
+evaluates to 
+
+    registers
+        r1 := x
+        r2 := y
+        r3 := x + y
+*)
+Example evaluate_intruction1 : 
+    interp_asm (denote_instr i1) mem startReg
+≋ 
+    result_i1.
+Proof.
+    (* first denote instruction 1 as an itree*)
+    unfold i1.
+    unfold denote_instr ; simpl.
+    (* then start interpreting the events *)
+    rewrite interp_asm_GetReg ; cbn.
+    rewrite interp_asm_GetReg; cbn.
+    rewrite interp_asm_SetReg'; cbn.
+    unfold startReg.
+
+    (* now all the events have been interpreted 
+        see if it equals the result *)
+    unfold result_i1; unfold endReg_i1 ; simpl;
+    unfold alist_add; unfold alist_remove; simpl.
+    (* the results match! *)
+    reflexivity.
+Qed.
+
+(* now we can finally show 
+i1: 
+    r3 := r1 + r2
+≋ 
+i2:
+    r3 := r3 + r1
+
+*)
+Theorem  bisimilar_i1_i2 : 
+    interp_asm (denote_instr i1) mem startReg
+≋   
+    interp_asm (denote_instr i2) mem startReg.
+Proof.
+    (* denote the instructions as itrees *)
+    unfold i1,i2 ; simpl.
+    (* interpret the events *)
+    eval_interp ; setoid_rewrite interp_asm_SetReg' ; cbn.
+    (* show that the register maps are equal 
+       we know that they are since addition is comutative
+    *)
+    setoid_rewrite plus_comm at 1.
+    (* now they are exactly equal! *)
+    reflexivity.
+Qed.
+
+End bisimilar_instruction.
