src/demo/exactEqBlocks.v
@@ -1,0 +1,178 @@
+From Coq Require Import
+Lists.List
+Strings.String
+Morphisms
+ZArith
+Setoid
+RelationClasses.
+
+(*Turning off some of the notation 
+helps to see what rules might be helpful*)
+
+From ITree Require Import
+    Eq.Eqit
+    Basics.Category
+    Basics.HeterogeneousRelations
+    Basics.Monad
+    Basics.CategorySub
+    Basics.CategoryOps
+    Interp.InterpFacts
+    Events.MapDefault
+    Events.MapDefaultFacts
+    Events.State
+    Events.StateFacts
+    ITreeMonad
+    ITreeFacts
+    ITree.
+
+From ExtLib Require Import
+    Core.RelDec
+    Structures.Monad
+    Structures.Maps
+    Programming.Show
+    Data.Map.FMapAList.
+
+Import CatNotations.
+Local Open Scope cat_scope.
+Local Open Scope itree_scope.
+
+From ITreeTutorial Require Import 
+    Fin 
+    Asm 
+    AsmCombinators 
+    AsmOptimization
+    Imp2Asm
+    KTreeFin
+    Utils_tutorial.
+
+Import ITreeNotations.
+
+Import ListNotations.
+Open Scope string_scope.
+
+Import CatNotations.
+Local Open Scope cat_scope.
+Local Open Scope itree_scope.
+
+From ITreeTutorial Require Import Fin Asm AsmCombinators Utils_tutorial.
+
+From MyProject Require Import 
+    Utils.
+
+
+Module exact_eq.
+Import utils.
+
+(* definition of two basic blocks *)
+
+(* 
+    bb0 : 
+        r1 := r1 + 1
+*)
+Definition bb0 : block (fin 1) := 
+    after [
+        Iadd 1 1 (Oimm 1)
+    ] (Bjmp f0).
+
+(* 
+    bb1 : 
+        r1 := r1 + 1
+*)
+Definition bb1 : block (fin 1) :=
+    after [
+        Iadd 1 1 (Oimm 1)
+    ] (Bjmp f0).
+
+Definition asm0 : asm 1 1 := raw_asm_block bb0.
+Definition asm1 : asm 1 1 := raw_asm_block bb1.
+
+(* summun an effect type for this example*)
+Notation E := Utils.utils.E.
+
+(* how about showing that asm0 and ams1 are bisimilar?
+   first we have to denote them as itrees *)
+Definition den_asm0 :itree E (fin 1) := denote_asm asm0 f0.
+Definition den_asm1 :itree E (fin 1) := denote_asm asm1 f0.
+
+
+
+(* This proof demonstrates that two exacly equal blocks are bilimilar*)
+Theorem ExactEqualBlocks : den_asm0 ≈ den_asm1.
+Proof.
+(* unfold definition of asm programs *)
+unfold den_asm0 ; unfold asm0.
+unfold den_asm1 ; unfold asm1.
+
+(*denote_asm (raw_asm_block b) f0 ≈ denote_bk b*)
+rewrite raw_asm_block_correct.
+rewrite raw_asm_block_correct.
+(* now we compute the denotation of bb0 and bb1 as 
+   interaction trees  *)
+unfold bb0.
+unfold bb1.
+setoid_rewrite denote_after.
+unfold denote_br .
+unfold denote_list.
+unfold denote_bk.
+unfold traverse_.
+unfold denote_instr.
+unfold denote_operand.
+simpl; repeat setoid_rewrite bind_bind.
+
+(* now that we've computed the denotation 
+   we can prove the bisimularity of itrees*)
+(* peel off  trigger (GetReg 1)*)
+eutt_clo_bind_eq.
+1:{ unfold trigger. 
+    apply eqit_Vis ;intros.
+    apply eqit_Ret.
+    reflexivity.
+} intros ; subst.
+
+(* peel off Ret 1*)
+eutt_clo_bind_eq.
+1:{
+    apply eqit_Ret.
+    reflexivity.
+ }
+intros; subst.
+
+(* peel off trigger (SetReg ...) *)
+unfold trigger ;setoid_rewrite bind_vis.
+eapply eqit_Vis ; intros.
+
+(* peel off Ret u*)
+eutt_clo_bind_eq.
+1:{ 
+    apply eqit_Ret.
+    reflexivity.
+} intros; subst.
+
+(* peel off Ret tt*)
+eutt_clo_bind_eq. 
+apply eqit_Ret ; reflexivity. 
+intros ; subst.
+
+(* finally we have Ret f0*)
+apply eqit_Ret.
+reflexivity.
+Qed.
+
+(* In that last example,
+    we manually computed the denotation 
+    and the bisimilarity of bb0 and bb1.
+    
+    Here is a much shorter proof.
+    *)
+Theorem short_ExactEqualBlocks : den_asm0 ≈ den_asm1.
+Proof.
+(* compute the denotation as itrees *)
+unfold den_asm0 ; unfold asm0 ; rewrite raw_asm_block_correct;
+unfold den_asm1 ; unfold asm1 ; rewrite raw_asm_block_correct;
+unfold denote_bk ; simpl.
+
+(* they are equal!*)
+reflexivity.
+Qed.
+
+End exact_eq.
